\begin{answer}
    $$
    \begin{aligned}
        \frac{\partial}{\partial \eta} \int p(y;\eta) dy &= \int \frac{\partial}{\partial \eta} p(y;\eta) dy\\
        &= \int \frac{\partial}{\partial \eta} b(y)\exp(\eta y - a(\eta))dy \\
        &= \int b(y)\exp(\eta y - a(\eta))(y - \frac{\partial}{\partial\eta}a(\eta))dy \\
        &= \int b(y)\exp(\eta y - a(\eta))y dy - \frac{\partial}{\partial\eta}a(\eta) \int b(y)\exp(\eta y - a(\eta))dy \\
        &= \int p(y;\eta)y dy - \frac{\partial}{\partial\eta}a(\eta) \int p(y;\eta)dy \\
        \text{note that $\int p(y;\eta) dy = 1$, so we have}\\
        0 &= \mathbb{E}[Y\mid X; \eta] - \frac{\partial}{\partial\eta}a(\eta) \\
        \mathbb{E}[Y\mid X; \eta] &= \frac{\partial}{\partial\eta}a(\eta)
    \end{aligned}
    $$
 
\end{answer}
