\begin{answer}
    $$
    \begin{aligned}
        p(y=1|x;\phi,\mu_0,\mu_1,\Sigma) &= \frac{p(x|y=1)p(y=1)}{p(x|y=0)p(y=0)+p(x|y=1)p(y=1)} \\
        &= \frac{1}{1+\frac{p(x|y=0)p(y=0)}{p(x|y=1)p(y=1)}} \\
        &= \frac{1}{1+\frac{1-\phi}{\phi}\exp{(\frac{1}{2}(x-\mu_1)^T\Sigma^{-1}(x-\mu_1) - \frac{1}{2}(x-\mu_0)^T\Sigma^{-1}(x-\mu_0)}} \\
        &=\frac{1}{1+\frac{1-\phi}{\phi}\exp{((\mu_0-\mu_1)^T\Sigma^{-1}x+\frac{1}{2}(\mu_1^T\Sigma^{-1}\mu_1 - }\mu_0^T\Sigma^{-1}\mu_0))}\\
        &=\frac{1}{1+\exp{\{-[(\mu_1-\mu_0)^T\Sigma^{-1}x+\frac{1}{2}(\mu_0^T\Sigma^{-1}\mu_0 - }\mu_1^T\Sigma^{-1}\mu_1)+\ln{(\frac{\phi}{1-\phi})}]\}}\\
        &=\frac{1}{1+\exp{(-(\theta^Tx+\theta_0))}}
        \end{aligned}\\
    $$
    note that $\Sigma$ is symmetric, so we have:
    $$
        \begin{aligned}
        \theta &= (\Sigma^{-1})^T(\mu_1-\mu_0) = \Sigma^{-1}(\mu_1-\mu_0)\\ 
        \theta_0 &=\frac{1}{2}(\mu_0^T\Sigma^{-1}\mu_0-\mu_1^T\Sigma^{-1}\mu_1)+\ln{\frac{\phi}{1-\phi}}
        \end{aligned}
    $$

\end{answer}
