\begin{answer}
    \begin{enumerate}
        \item 
        $$
        \begin{aligned}
            \theta^{(i+1)} :&=\theta^{(i)} + \alpha \left(y^{(i+1)} - h_{\theta^{(i)}}(\phi(x^{(i+1)}))\right) \phi(x^{(i+1)})\\
            \theta^{(i)} &= \sum_{j = 1}^i\beta_j\phi(x^{(j)}) \\
            \theta^{(0)} &= \vec{0} \\
        \end{aligned}
        $$
        \item 
        $$
        \begin{aligned}
            h_{\theta^{(i)}}(x^{(i+1)}) &= g\left({\theta^{(i)}}^T \phi(x^{(i+1)})\right)\\
            &= g\left( \sum_{j = 1}^i\beta_j\phi(x^{(j)}) \cdot \phi(x^{(i+1)}) \right) \\
            &= g\left( \sum_{j = 1}^i\beta_j K(x^{(j)}, x^{(i+1)})\right) \\
        \end{aligned}
        $$
        \item 
        $$
        \begin{aligned}
            \theta^{(i+1)} &:= \theta^{(i)} + \alpha (y^{(i+1)} - h_{\theta^{(i)}}(x^{(i+1)})) \phi(x^{(i+1)})         \\
            \theta^{(i+1)} &:= \sum_{j = 1}^i\beta_j\phi(x^{(j)}) + \alpha (y^{(i+1)} - g( \sum_{j = 1}^i\beta_j K(x^{(j)}, x^{(i+1)})) \phi(x^{(i+1)})         \\
            \sum_{j = 1}^{i+1}\beta_j\phi(x^{(j)}) &:= \sum_{j = 1}^i\beta_j\phi(x^{(j)}) + \alpha (y^{(i+1)} - g( \sum_{j = 1}^i\beta_j K(x^{(j)}, x^{(i+1)})) \phi(x^{(i+1)})         \\
            \beta_{i+1} &:= \alpha (y^{(i+1)} - g( \sum_{j = 1}^i\beta_j K(x^{(j)}, x^{(i+1)}))       \\
        \end{aligned}
        $$
    \end{enumerate}
\end{answer}
