\begin{answer}
    
    exponential family can be written in the form:
    $$
        p(y; \eta) = b(y)\exp{(\eta^TT(y)-a(\eta))}
    $$
    note that:
    $$
            p(y; \lambda) = \frac{e^{-\lambda}\lambda^y}{y!}
            =\frac{1}{y!}\exp(y\ln{\lambda}-\lambda)
    $$
    therefore, 
    $$
    \begin{aligned}
        \eta    &= \ln{\lambda} \\
        T(y)    &= y \\
        a(\eta) &= \lambda \\
                &= e^{\eta}\\
            b(y)&=\frac{1}{y!}
    \end{aligned}
    $$
\end{answer}
