\begin{answer}
    $$
    \begin{aligned}
        p(t^{(i)}=1 \mid x_{(i)}) &= \frac{p(y^{(i)}=1 \mid x_{(i)})}{\alpha}\\
        \frac{p(t^{(i)}=1 , x_{(i)})}{p(x^{(i)})} &= \frac{p(y^{(i)}=1 , x_{(i)})}{\alpha p(x^{(i)})} \\
        \alpha &= \frac{p(y^{(i)}=1 , x_{(i)})}{p(t^{(i)}=1 , x_{(i)})}
    \end{aligned}
    $$
    note that $p(t^{(i)}=1\mid y^{(i)}=1) = 1$, i.e. $p(t^{(i)}=1, y^{(i)}=1)=p(y^{(i)}=1)$, then:\\
    $$
    \begin{aligned}
        p(y^{(i)} = 1\mid t^{(i)} = 1, x^{(i)}) &= p(y^{(i)} = 1\mid t^{(i)} = 1) \\
        \frac{p(y^{(i)} = 1, t^{(i)} = 1, x^{(i)})}{p(t^{(i)} = 1, x^{(i)}) } &= \frac{p(y^{(i)} = 1, t^{(i)} = 1)}{p(t^{(i)} = 1)}\\
        \frac{p(y^{(i)} = 1, x^{(i)})}{p(t^{(i)} = 1, x^{(i)}) } &= \frac{p(y^{(i)} = 1)}{p(t^{(i)} = 1)}\\
    \end{aligned}
    $$
    so we have $\alpha = \frac{p(y^{(i)} = 1)}{p(t^{(i)} = 1)}$, and is constant. 
\end{answer}
